More logic stuff

Logic/Propositional/Linear/Intuitionistic.lean
@@ -1,5 +1,3 @@
-namespace Logic.Propositional.Linear.Intuitionistic
-
 opaque BasePropn : Type
 
 inductive Propn
@@ -14,230 +12,191 @@ inductive Propn
 
 inductive Ctx
   | nil
-  | cons (Γ : Ctx) (A : Propn)
+  | cons (Δ : Ctx) (A : Propn)
 
-def Ctx.append (Γ : Ctx) : (Γ' : Ctx) → Ctx
-  | nil => Γ
-  | cons Γ' A => (Γ.append Γ').cons A
-
-theorem Ctx.nil_append : ∀ {Γ}, nil.append Γ = Γ
-  | nil => rfl
-  | cons .. => congrArg (cons · _) nil_append
-
-theorem Ctx.append_append : ∀ {Γ''}, append Γ (Γ'.append Γ'') = (Γ.append Γ').append Γ''
-  | nil => rfl
-  | cons .. => congrArg (cons · _) append_append
-
-inductive Split : (Γ Γ₁ Γ₂ : Ctx) → Type
+inductive Split : (Δ Δ₁ Δ₂ : Ctx) → Type
   | nil : Split .nil .nil .nil
-  | cons₁ (s : Split Γ Γ₁ Γ₂) : Split (Γ.cons A) (Γ₁.cons A) Γ₂
-  | cons₂ (s : Split Γ Γ₁ Γ₂) : Split (Γ.cons A) Γ₁ (Γ₂.cons A)
+  | cons₁ (s : Split Δ Δ₁ Δ₂) : Split (Δ.cons A) (Δ₁.cons A) Δ₂
+  | cons₂ (s : Split Δ Δ₁ Δ₂) : Split (Δ.cons A) Δ₁ (Δ₂.cons A)
 
-def Split.triv₁ : ∀ {Γ}, Split Γ Γ .nil
+def Split.triv₁ : ∀ {Δ}, Split Δ Δ .nil
   | .nil => nil
   | .cons .. => triv₁.cons₁
 
-def Split.triv₂ : ∀ {Γ}, Split Γ .nil Γ
+def Split.triv₂ : ∀ {Δ}, Split Δ .nil Δ
   | .nil => nil
   | .cons .. => triv₂.cons₂
 
-theorem Split.eq_triv₁ : ∀ s, (⟨Γ₁, s⟩ : Σ Γ₁, Split Γ Γ₁ .nil) = ⟨Γ, triv₁⟩
+theorem Split.eq_triv₁ : ∀ s, (⟨Δ₁, s⟩ : Σ Δ₁, Split Δ Δ₁ .nil) = ⟨Δ, triv₁⟩
   | nil => rfl
   | cons₁ s => let .refl _ := s.eq_triv₁; rfl
 
-theorem Split.eq_triv₂ : ∀ s, (⟨Γ₂, s⟩ : Σ Γ₂, Split Γ .nil Γ₂) = ⟨Γ, triv₂⟩
+theorem Split.eq_triv₂ : ∀ s, (⟨Δ₂, s⟩ : Σ Δ₂, Split Δ .nil Δ₂) = ⟨Δ, triv₂⟩
   | nil => rfl
   | cons₂ s => let .refl _ := s.eq_triv₂; rfl
 
-def Split.flip : (s : Split Γ Γ₁ Γ₂) → Split Γ Γ₂ Γ₁
+def Split.flip : (s : Split Δ Δ₁ Δ₂) → Split Δ Δ₂ Δ₁
   | nil => nil
   | cons₁ s => s.flip.cons₂
   | cons₂ s => s.flip.cons₁
 
-def Split.shift₁ : (s : Split Γ Γ₁ Γ₂) → (s₁ : Split Γ₁ Γ₁₁ Γ₁₂) → Σ Γ', Split Γ Γ₁₁ Γ' × Split Γ' Γ₁₂ Γ₂
+def Split.shift₁ : (s : Split Δ Δ₁ Δ₂) → (s₁ : Split Δ₁ Δ₁₁ Δ₁₂) → Σ Δ', Split Δ Δ₁₁ Δ' × Split Δ' Δ₁₂ Δ₂
   | s, nil => ⟨_, triv₂, s⟩
   | cons₁ s, cons₁ s₁ => let ⟨_, s, s'⟩ := s.shift₁ s₁; ⟨_, s.cons₁, s'⟩
   | cons₁ s, cons₂ s₁ => let ⟨_, s, s'⟩ := s.shift₁ s₁; ⟨_, s.cons₂, s'.cons₁⟩
   | cons₂ s, s₁ => let ⟨_, s, s'⟩ := s.shift₁ s₁; ⟨_, s.cons₂, s'.cons₂⟩
 
-def Split.mkAppend : ∀ {Γ₂}, Split (Γ₁.append Γ₂) Γ₁ Γ₂
-  | .nil => triv₁
-  | .cons .. => mkAppend.cons₂
-
-def Split.append₂ (s : Split Γ Γ₁ Γ₂) : ∀ {Γ'}, Split (Γ.append Γ') Γ₁ (Γ₂.append Γ')
-  | .nil => s
-  | .cons .. => s.append₂.cons₂
-
-def Split.append₂' : (s : Split Γ Γ₁ Γ₂) → ∀ {Γ'}, Split (.append Γ' Γ) Γ₁ (Γ'.append Γ₂)
-  | nil => triv₂
-  | cons₁ s => s.append₂'.cons₁
-  | cons₂ s => s.append₂'.cons₂
-
-inductive Subst (J : (Γ : Ctx) → (A : Propn) → Type) : (Γ Γ' : Ctx) → Type
+inductive Subst (J : (Δ : Ctx) → (A : Propn) → Type) : (Δ Δ' : Ctx) → Type
   | nil : Subst J .nil .nil
-  | cons (s : Split Γ' Γ₁ Γ₂) (D : J Γ₁ A) (γ : Subst J Γ Γ₂) : Subst J (Γ.cons A) Γ'
+  | cons (s : Split Δ' Δ₁ Δ₂) (D : J Δ₁ A) (δ : Subst J Δ Δ₂) : Subst J (Δ.cons A) Δ'
 
-def Subst.split : (γ : Subst J Γ Γ') → ∀ {Γ₁ Γ₂}, (s : Split Γ Γ₁ Γ₂) → Σ Γ₁' Γ₂', Split Γ' Γ₁' Γ₂' × Subst J Γ₁ Γ₁' × Subst J Γ₂ Γ₂'
+def Subst.split : (δ : Subst J Δ Δ') → ∀ {Δ₁ Δ₂}, (s : Split Δ Δ₁ Δ₂) → Σ Δ₁' Δ₂', Split Δ' Δ₁' Δ₂' × Subst J Δ₁ Δ₁' × Subst J Δ₂ Δ₂'
   | nil, _, _, .nil => ⟨_, _, .nil, nil, nil⟩
-  | cons s' D γ, _, _, .cons₁ s => let ⟨_, _, s, γ₁, γ₂⟩ := γ.split s; let ⟨_, s, s'⟩ := s'.flip.shift₁ s.flip; ⟨_, _, s.flip, cons s'.flip D γ₁, γ₂⟩
-  | cons s' D γ, _, _, .cons₂ s => let ⟨_, _, s, γ₁, γ₂⟩ := γ.split s; let ⟨_, s, s'⟩ := s'.flip.shift₁ s; ⟨_, _, s, γ₁, cons s'.flip D γ₂⟩
+  | cons s' D δ, _, _, .cons₁ s => let ⟨_, _, s, δ₁, δ₂⟩ := δ.split s; let ⟨_, s, s'⟩ := s'.flip.shift₁ s.flip; ⟨_, _, s.flip, cons s'.flip D δ₁, δ₂⟩
+  | cons s' D δ, _, _, .cons₂ s => let ⟨_, _, s, δ₁, δ₂⟩ := δ.split s; let ⟨_, s, s'⟩ := s'.flip.shift₁ s; ⟨_, _, s, δ₁, cons s'.flip D δ₂⟩
 
-def Subst.append (γ₁ : Subst J Γ₁ Γ₁') : (γ₂ : Subst J Γ₂ Γ₂') → Subst J (Γ₁.append Γ₂) (Γ₁'.append Γ₂')
-  | nil => γ₁
-  | cons s D γ₂ => cons s.append₂' D (γ₁.append γ₂)
-
-def Subst.consAppend (D : J (.cons .nil A) A) : ∀ {Γ₂}, (γ : Subst J (.append Γ₁ Γ₂) Γ') → Subst J ((Γ₁.cons A).append Γ₂) (Γ'.cons A)
-  | .nil, γ => cons (.cons₁ .triv₂) D γ
-  | .cons .., cons s D' γ => cons s.cons₂ D' (γ.consAppend D)
-
-inductive Hyp : (Γ : Ctx) → (A : Propn) → Type
+inductive Hyp : (Δ : Ctx) → (A : Propn) → Type
   | mk : Hyp (.cons .nil A) A
 
-def Split.toSubst : (s : Split Γ Γ₁ Γ₂) → Subst Hyp (Γ₁.append Γ₂) Γ
-  | nil => .nil
-  | cons₁ s => .consAppend .mk s.toSubst
-  | cons₂ s => .cons triv₂.cons₁ .mk s.toSubst
+class Judge (J : (Δ : Ctx) → (A : Propn) → Type) where
+  hyp : J (.cons .nil A) A
 
-class JudgeTrans (J J' : (Γ : Ctx) → (A : Propn) → Type) where
-  transform (D : J Γ A) : J' Γ A
+instance Hyp.judge : Judge Hyp where
+  hyp := mk
 
-instance JudgeTrans.id : JudgeTrans J J where
-  transform D := D
-
-abbrev Judge : (J : (Γ : Ctx) → (A : Propn) → Type) → Type :=
-  JudgeTrans Hyp
-
-def Subst.id [j : Judge J] : ∀ {Γ}, Subst J Γ Γ
+def Subst.id [j : Judge J] : ∀ {Δ}, Subst J Δ Δ
   | .nil => nil
-  | .cons .. => cons (.cons₁ .triv₂) (j.transform .mk) id
+  | .cons .. => cons (.cons₁ .triv₂) j.hyp id
 
-def Subst.lift [j : Judge J] {Γ Γ' A} : (γ : Subst J Γ Γ') → Subst J (Γ.cons A) (Γ'.cons A) :=
-  cons (.cons₁ .triv₂) (j.transform .mk)
+def Subst.lift [j : Judge J] {Δ Δ' A} : (δ : Subst J Δ Δ') → Subst J (Δ.cons A) (Δ'.cons A) :=
+  cons (.cons₁ .triv₂) j.hyp
 
-def Subst.map (jt : JudgeTrans J J') {Γ Γ'} : (γ : Subst J Γ Γ') → Subst J' Γ Γ'
+def Subst.map (f : ∀ {Δ A}, (D : J Δ A) → J' Δ A) {Δ Δ'} : (δ : Subst J Δ Δ') → Subst J' Δ Δ'
   | nil => nil
-  | cons s D γ => cons s (jt.transform D) (γ.map jt)
+  | cons s D δ => cons s (f D) (δ.map @f)
 
-def Subst.exchange : Subst Hyp (Ctx.cons Γ A |>.cons B) (Γ.cons B |>.cons A) :=
+def Subst.exchange : Subst Hyp (Ctx.cons Δ A |>.cons B) (Δ.cons B |>.cons A) :=
   cons (.cons₂ (.cons₁ .triv₂)) .mk id
 
-def Subst.exchange₂ : Subst Hyp (Ctx.cons Γ A |>.cons B |>.cons C) (Γ.cons B |>.cons C |>.cons A) :=
+def Subst.exchange₂ : Subst Hyp (Ctx.cons Δ A |>.cons B |>.cons C) (Δ.cons B |>.cons C |>.cons A) :=
   cons (.cons₂ (.cons₁ .triv₂)) .mk exchange
 
-inductive Split₁ : (Γ : Ctx) → (A : Propn) → (Γ' : Ctx) → Type
-  | here : Split₁ (Γ.cons A) A Γ
-  | there (s : Split₁ Γ A Γ') : Split₁ (Γ.cons B) A (Γ'.cons B)
+inductive Split₁ : (Δ : Ctx) → (A : Propn) → (Δ' : Ctx) → Type
+  | here : Split₁ (Δ.cons A) A Δ
+  | there (s : Split₁ Δ A Δ') : Split₁ (Δ.cons B) A (Δ'.cons B)
 
-def Split₁.toSplit : (s : Split₁ Γ A Γ') → Split Γ (.cons .nil A) Γ'
+def Split₁.toSplit : (s : Split₁ Δ A Δ') → Split Δ (.cons .nil A) Δ'
   | here => .cons₁ .triv₂
   | there s => s.toSplit.cons₂
 
-def Split₁.ofSplit : (s : Split Γ (.cons .nil A) Γ') → Split₁ Γ A Γ'
+def Split₁.ofSplit : (s : Split Δ (.cons .nil A) Δ') → Split₁ Δ A Δ'
   | .cons₁ s => let .refl _ := s.eq_triv₂; here
   | .cons₂ s => (ofSplit s).there
 
-def Subst.split₁ (γ : Subst Hyp Γ Γ') {A Γ₂} (s : Split₁ Γ A Γ₂) : Σ Γ₂', Split₁ Γ' A Γ₂' × Subst Hyp Γ₂ Γ₂' :=
-  let ⟨_, _, s, cons s' .mk nil, γ⟩ := γ.split s.toSplit
-  let .cons₁ .nil := s'
-  ⟨_, .ofSplit s, γ⟩
+def Subst.split₁ (δ : Subst J Δ Δ') {A Δ₂} (s : Split₁ Δ A Δ₂) : Σ Δ₁' Δ₂', Split Δ' Δ₁' Δ₂' × J Δ₁' A × Subst J Δ₂ Δ₂' :=
+  let ⟨_, _, s, cons s' D nil, δ⟩ := δ.split s.toSplit
+  let .refl _ := s'.eq_triv₁
+  ⟨_, _, s, D, δ⟩
 
--- Natural Deduction
+/-! Natural Deduction -/
+
 namespace ND
 
-inductive True : (Γ : Ctx) → (A : Propn) → Type
+inductive True : (Δ : Ctx) → (A : Propn) → Type
   | hyp : True (.cons .nil A) A
   | oneI : True .nil .one
-  | oneE (s : Split Γ Γ₁ Γ₂) (D : True Γ₁ .one) (D₁ : True Γ₂ C) : True Γ C
-  | zeroE (s : Split Γ Γ₁ Γ₂) (D : True Γ₁ .zero) : True Γ C
-  | topI : True Γ .top
-  | tensorI (s : Split Γ Γ₁ Γ₂) (D₁ : True Γ₁ A) (D₂ : True Γ₂ B) : True Γ (A.tensor B)
-  | tensorE (s : Split Γ Γ₁ Γ₂) (D : True Γ₁ (A.tensor B)) (D₁ : True (Γ₂.cons A |>.cons B) C) : True Γ C
-  | plusI₁ (D : True Γ A) : True Γ (A.plus B)
-  | plusI₂ (D : True Γ B) : True Γ (.plus A B)
-  | plusE (s : Split Γ Γ₁ Γ₂) (D : True Γ₁ (A.plus B)) (D₁ : True (Γ₂.cons A) C) (D₂ : True (Γ₂.cons B) C) : True Γ C
-  | withI (D₁ : True Γ A) (D₂ : True Γ B) : True Γ (A.with B)
-  | withE₁ (D : True Γ (A.with B)) : True Γ A
-  | withE₂ (D : True Γ (.with A B)) : True Γ B
-  | lolliI (D : True (Γ.cons A) B) : True Γ (A.lolli B)
-  | lolliE (s : Split Γ Γ₁ Γ₂) (D : True Γ₁ (A.lolli B)) (D₁ : True Γ₂ A) : True Γ B
+  | oneE (s : Split Δ Δ₁ Δ₂) (D : True Δ₁ .one) (D₁ : True Δ₂ C) : True Δ C
+  | zeroE (s : Split Δ Δ₁ Δ₂) (D : True Δ₁ .zero) : True Δ C
+  | topI : True Δ .top
+  | tensorI (s : Split Δ Δ₁ Δ₂) (D₁ : True Δ₁ A) (D₂ : True Δ₂ B) : True Δ (A.tensor B)
+  | tensorE (s : Split Δ Δ₁ Δ₂) (D : True Δ₁ (A.tensor B)) (D₁ : True (Δ₂.cons A |>.cons B) C) : True Δ C
+  | plusI₁ (D : True Δ A) : True Δ (A.plus B)
+  | plusI₂ (D : True Δ B) : True Δ (.plus A B)
+  | plusE (s : Split Δ Δ₁ Δ₂) (D : True Δ₁ (A.plus B)) (D₁ : True (Δ₂.cons A) C) (D₂ : True (Δ₂.cons B) C) : True Δ C
+  | withI (D₁ : True Δ A) (D₂ : True Δ B) : True Δ (A.with B)
+  | withE₁ (D : True Δ (A.with B)) : True Δ A
+  | withE₂ (D : True Δ (.with A B)) : True Δ B
+  | lolliI (D : True (Δ.cons A) B) : True Δ (A.lolli B)
+  | lolliE (s : Split Δ Δ₁ Δ₂) (D : True Δ₁ (A.lolli B)) (D₁ : True Δ₂ A) : True Δ B
 
 instance True.judge : Judge True where
-  transform | .mk => hyp
+  hyp := hyp
 
-def True.subst [j : Judge J] [jt : JudgeTrans J True] {Γ Γ'} (γ : Subst J Γ Γ') {A} : (D : True Γ A) → True Γ' A
-  | hyp => let .cons s D .nil := γ; let .refl _ := s.eq_triv₁; jt.transform D
-  | oneI => let .nil := γ; oneI
-  | oneE s D D₁ => let ⟨_, _, s, γ₁, γ₂⟩ := γ.split s; oneE s (D.subst γ₁) (D₁.subst γ₂)
-  | zeroE s D => let ⟨_, _, s, γ₁, _⟩ := γ.split s; zeroE s (D.subst γ₁)
+def True.subst (δ : Subst True Δ Δ') {A} : (D : True Δ A) → True Δ' A
+  | hyp => let .cons s D .nil := δ; let .refl _ := s.eq_triv₁; D
+  | oneI => let .nil := δ; oneI
+  | oneE s D D₁ => let ⟨_, _, s, δ₁, δ₂⟩ := δ.split s; oneE s (D.subst δ₁) (D₁.subst δ₂)
+  | zeroE s D => let ⟨_, _, s, δ₁, _⟩ := δ.split s; zeroE s (D.subst δ₁)
   | topI => topI
-  | tensorI s D₁ D₂ => let ⟨_, _, s, γ₁, γ₂⟩ := γ.split s; tensorI s (D₁.subst γ₁) (D₂.subst γ₂)
-  | tensorE s D D₁ => let ⟨_, _, s, γ₁, γ₂⟩ := γ.split s; tensorE s (D.subst γ₁) (D₁.subst γ₂.lift.lift)
-  | plusI₁ D => plusI₁ (D.subst γ)
-  | plusI₂ D => plusI₂ (D.subst γ)
-  | plusE s D D₁ D₂ => let ⟨_, _, s, γ₁, γ₂⟩ := γ.split s; plusE s (D.subst γ₁) (D₁.subst γ₂.lift) (D₂.subst γ₂.lift)
-  | withI D₁ D₂ => withI (D₁.subst γ) (D₂.subst γ)
-  | withE₁ D => withE₁ (D.subst γ)
-  | withE₂ D => withE₂ (D.subst γ)
-  | lolliI D => lolliI (D.subst γ.lift)
-  | lolliE s D D₁ => let ⟨_, _, s, γ₁, γ₂⟩ := γ.split s; lolliE s (D.subst γ₁) (D₁.subst γ₂)
+  | tensorI s D₁ D₂ => let ⟨_, _, s, δ₁, δ₂⟩ := δ.split s; tensorI s (D₁.subst δ₁) (D₂.subst δ₂)
+  | tensorE s D D₁ => let ⟨_, _, s, δ₁, δ₂⟩ := δ.split s; tensorE s (D.subst δ₁) (D₁.subst δ₂.lift.lift)
+  | plusI₁ D => plusI₁ (D.subst δ)
+  | plusI₂ D => plusI₂ (D.subst δ)
+  | plusE s D D₁ D₂ => let ⟨_, _, s, δ₁, δ₂⟩ := δ.split s; plusE s (D.subst δ₁) (D₁.subst δ₂.lift) (D₂.subst δ₂.lift)
+  | withI D₁ D₂ => withI (D₁.subst δ) (D₂.subst δ)
+  | withE₁ D => withE₁ (D.subst δ)
+  | withE₂ D => withE₂ (D.subst δ)
+  | lolliI D => lolliI (D.subst δ.lift)
+  | lolliE s D D₁ => let ⟨_, _, s, δ₁, δ₂⟩ := δ.split s; lolliE s (D.subst δ₁) (D₁.subst δ₂)
 
 end ND
 
--- Verifications and Uses
+/-! Verifications and Uses -/
+
 namespace VU
 
 mutual
 
-inductive Verif : (Γ : Ctx) → (A : Propn) → Type
-  | uv (D : Use Γ (.base P)) : Verif Γ (.base P)
+inductive Verif : (Δ : Ctx) → (A : Propn) → Type
+  | uv (D : Use Δ (.base P)) : Verif Δ (.base P)
   | oneI : Verif .nil .one
-  | oneE (s : Split Γ Γ₁ Γ₂) (D : Use Γ₁ .one) (D₁ : Verif Γ₂ C) : Verif Γ C
-  | zeroE (s : Split Γ Γ₁ Γ₂) (D : Use Γ₁ .zero) : Verif Γ C
-  | topI : Verif Γ .top
-  | tensorI (s : Split Γ Γ₁ Γ₂) (D₁ : Verif Γ₁ A) (D₂ : Verif Γ₂ B) : Verif Γ (A.tensor B)
-  | tensorE (s : Split Γ Γ₁ Γ₂) (D : Use Γ₁ (A.tensor B)) (D₁ : Verif (Γ₂.cons A |>.cons B) C) : Verif Γ C
-  | plusI₁ (D : Verif Γ A) : Verif Γ (A.plus B)
-  | plusI₂ (D : Verif Γ B) : Verif Γ (.plus A B)
-  | plusE (s : Split Γ Γ₁ Γ₂) (D : Use Γ₁ (A.plus B)) (D₁ : Verif (Γ₂.cons A) C) (D₂ : Verif (Γ₂.cons B) C) : Verif Γ C
-  | withI (D₁ : Verif Γ A) (D₂ : Verif Γ B) : Verif Γ (A.with B)
-  | lolliI (D : Verif (Γ.cons A) B) : Verif Γ (A.lolli B)
+  | oneE (s : Split Δ Δ₁ Δ₂) (D : Use Δ₁ .one) (D₁ : Verif Δ₂ C) : Verif Δ C
+  | zeroE (s : Split Δ Δ₁ Δ₂) (D : Use Δ₁ .zero) : Verif Δ C
+  | topI : Verif Δ .top
+  | tensorI (s : Split Δ Δ₁ Δ₂) (D₁ : Verif Δ₁ A) (D₂ : Verif Δ₂ B) : Verif Δ (A.tensor B)
+  | tensorE (s : Split Δ Δ₁ Δ₂) (D : Use Δ₁ (A.tensor B)) (D₁ : Verif (Δ₂.cons A |>.cons B) C) : Verif Δ C
+  | plusI₁ (D : Verif Δ A) : Verif Δ (A.plus B)
+  | plusI₂ (D : Verif Δ B) : Verif Δ (.plus A B)
+  | plusE (s : Split Δ Δ₁ Δ₂) (D : Use Δ₁ (A.plus B)) (D₁ : Verif (Δ₂.cons A) C) (D₂ : Verif (Δ₂.cons B) C) : Verif Δ C
+  | withI (D₁ : Verif Δ A) (D₂ : Verif Δ B) : Verif Δ (A.with B)
+  | lolliI (D : Verif (Δ.cons A) B) : Verif Δ (A.lolli B)
 
-inductive Use : (Γ : Ctx) → (A : Propn) → Type
+inductive Use : (Δ : Ctx) → (A : Propn) → Type
   | hyp : Use (.cons .nil A) A
-  | withE₁ (D : Use Γ (A.with B)) : Use Γ A
-  | withE₂ (D : Use Γ (.with A B)) : Use Γ B
-  | lolliE (s : Split Γ Γ₁ Γ₂) (D : Use Γ₁ (A.lolli B)) (D₁ : Verif Γ₂ A) : Use Γ B
+  | withE₁ (D : Use Δ (A.with B)) : Use Δ A
+  | withE₂ (D : Use Δ (.with A B)) : Use Δ B
+  | lolliE (s : Split Δ Δ₁ Δ₂) (D : Use Δ₁ (A.lolli B)) (D₁ : Verif Δ₂ A) : Use Δ B
 
 end
 
 instance Use.judge : Judge Use where
-  transform | .mk => hyp
+  hyp := hyp
 
 mutual
 
-def Verif.subst [j : Judge J] [jt : JudgeTrans J Use] {Γ Γ'} (γ : Subst J Γ Γ') {A} : (D : Verif Γ A) → Verif Γ' A
-  | .uv D => .uv (D.subst γ)
-  | .oneI => let .nil := γ; .oneI
-  | .oneE s D D₁ => let ⟨_, _, s, γ₁, γ₂⟩ := γ.split s; .oneE s (D.subst γ₁) (D₁.subst γ₂)
-  | .zeroE s D => let ⟨_, _, s, γ₁, _⟩ := γ.split s; .zeroE s (D.subst γ₁)
+def Verif.subst {Δ Δ'} (δ : Subst Use Δ Δ') {A} : (D : Verif Δ A) → Verif Δ' A
+  | .uv D => .uv (D.subst δ)
+  | .oneI => let .nil := δ; .oneI
+  | .oneE s D D₁ => let ⟨_, _, s, δ₁, δ₂⟩ := δ.split s; .oneE s (D.subst δ₁) (D₁.subst δ₂)
+  | .zeroE s D => let ⟨_, _, s, δ₁, _⟩ := δ.split s; .zeroE s (D.subst δ₁)
   | .topI => .topI
-  | .tensorI s D₁ D₂ => let ⟨_, _, s, γ₁, γ₂⟩ := γ.split s; .tensorI s (D₁.subst γ₁) (D₂.subst γ₂)
-  | .tensorE s D D₁ => let ⟨_, _, s, γ₁, γ₂⟩ := γ.split s; .tensorE s (D.subst γ₁) (D₁.subst γ₂.lift.lift)
-  | .plusI₁ D => .plusI₁ (D.subst γ)
-  | .plusI₂ D => .plusI₂ (D.subst γ)
-  | .plusE s D D₁ D₂ => let ⟨_, _, s, γ₁, γ₂⟩ := γ.split s; .plusE s (D.subst γ₁) (D₁.subst γ₂.lift) (D₂.subst γ₂.lift)
-  | .withI D₁ D₂ => .withI (D₁.subst γ) (D₂.subst γ)
-  | .lolliI D => .lolliI (D.subst γ.lift)
+  | .tensorI s D₁ D₂ => let ⟨_, _, s, δ₁, δ₂⟩ := δ.split s; .tensorI s (D₁.subst δ₁) (D₂.subst δ₂)
+  | .tensorE s D D₁ => let ⟨_, _, s, δ₁, δ₂⟩ := δ.split s; .tensorE s (D.subst δ₁) (D₁.subst δ₂.lift.lift)
+  | .plusI₁ D => .plusI₁ (D.subst δ)
+  | .plusI₂ D => .plusI₂ (D.subst δ)
+  | .plusE s D D₁ D₂ => let ⟨_, _, s, δ₁, δ₂⟩ := δ.split s; .plusE s (D.subst δ₁) (D₁.subst δ₂.lift) (D₂.subst δ₂.lift)
+  | .withI D₁ D₂ => .withI (D₁.subst δ) (D₂.subst δ)
+  | .lolliI D => .lolliI (D.subst δ.lift)
 
-def Use.subst [j : Judge J] [jt : JudgeTrans J Use] {Γ Γ'} (γ : Subst J Γ Γ') {A} : (D : Use Γ A) → Use Γ' A
-  | .hyp => let .cons s D .nil := γ; let .refl _ := s.eq_triv₁; jt.transform D
-  | .withE₁ D => .withE₁ (D.subst γ)
-  | .withE₂ D => .withE₂ (D.subst γ)
-  | .lolliE s D D₁ => let ⟨_, _, s, γ₁, γ₂⟩ := γ.split s; .lolliE s (D.subst γ₁) (D₁.subst γ₂)
+def Use.subst {Δ Δ'} (δ : Subst Use Δ Δ') {A} : (D : Use Δ A) → Use Δ' A
+  | .hyp => let .cons s D .nil := δ; let .refl _ := s.eq_triv₁; D
+  | .withE₁ D => .withE₁ (D.subst δ)
+  | .withE₂ D => .withE₂ (D.subst δ)
+  | .lolliE s D D₁ => let ⟨_, _, s, δ₁, δ₂⟩ := δ.split s; .lolliE s (D.subst δ₁) (D₁.subst δ₂)
 
 end
 
-def Verif.uv' (D : Use Γ A) : Verif Γ A :=
+def Verif.uv' (D : Use Δ A) : Verif Δ A :=
   match A with
   | .base _ => uv D
   | .one => oneE .triv₁ D oneI
@@ -249,11 +208,11 @@ def Verif.uv' (D : Use Γ A) : Verif Γ A :=
   | .lolli .. => lolliI (uv' (.lolliE (.cons₂ .triv₁) D (uv' .hyp)))
 
 instance Verif.judge : Judge Verif where
-  transform | .mk => uv' .hyp
+  hyp := uv' .hyp
 
 mutual
 
-def Verif.toTrue : (D : Verif Γ A) → ND.True Γ A
+def Verif.toTrue : (D : Verif Δ A) → ND.True Δ A
   | .uv D => D.toTrue
   | .oneI => .oneI
   | .oneE s D D₁ => .oneE s D.toTrue D₁.toTrue
@@ -267,7 +226,7 @@ def Verif.toTrue : (D : Verif Γ A) → ND.True Γ A
   | .withI D₁ D₂ => .withI D₁.toTrue D₂.toTrue
   | .lolliI D => .lolliI D.toTrue
 
-def Use.toTrue : (D : Use Γ A) → ND.True Γ A
+def Use.toTrue : (D : Use Δ A) → ND.True Δ A
   | .hyp => .hyp
   | .withE₁ D => .withE₁ D.toTrue
   | .withE₂ D => .withE₂ D.toTrue
@@ -277,42 +236,49 @@ end
 
 end VU
 
--- Sequent Calculus
-namespace SC
+/-! Sequent Calculus -/
 
-inductive Seq : (Γ : Ctx) → (A : Propn) → Type
+inductive SC.Seq : (Δ : Ctx) → (A : Propn) → Type
   | id : Seq (.cons .nil (.base P)) (.base P)
   | oneR : Seq .nil .one
-  | oneL (s : Split₁ Γ .one Γ') (D : Seq Γ' C) : Seq Γ C
-  | zeroL (s : Split₁ Γ .zero Γ') : Seq Γ C
-  | topR : Seq Γ .top
-  | tensorR (s : Split Γ Γ₁ Γ₂) (D₁ : Seq Γ₁ A) (D₂ : Seq Γ₂ B) : Seq Γ (A.tensor B)
-  | tensorL (s : Split₁ Γ (A.tensor B) Γ') (D : Seq (Γ'.cons A |>.cons B) C) : Seq Γ C
-  | plusR₁ (D : Seq Γ A) : Seq Γ (A.plus B)
-  | plusR₂ (D : Seq Γ B) : Seq Γ (.plus A B)
-  | plusL (s : Split₁ Γ (A.plus B) Γ') (D₁ : Seq (Γ'.cons A) C) (D₂ : Seq (Γ'.cons B) C) : Seq Γ C
-  | withR (D₁ : Seq Γ A) (D₂ : Seq Γ B) : Seq Γ (A.with B)
-  | withL₁ (s : Split₁ Γ (A.with B) Γ') (D : Seq (Γ'.cons A) C) : Seq Γ C
-  | withL₂ (s : Split₁ Γ (.with A B) Γ') (D : Seq (Γ'.cons B) C) : Seq Γ C
-  | lolliR (D : Seq (Γ.cons A) B) : Seq Γ (A.lolli B)
-  | lolliL (s : Split₁ Γ (A.lolli B) Γ') (s' : Split Γ' Γ₁ Γ₂) (D₁ : Seq Γ₁ A) (D₂ : Seq (Γ₂.cons B) C) : Seq Γ C
+  | oneL (s : Split₁ Δ .one Δ') (D : Seq Δ' C) : Seq Δ C
+  | zeroL (s : Split₁ Δ .zero Δ') : Seq Δ C
+  | topR : Seq Δ .top
+  | tensorR (s : Split Δ Δ₁ Δ₂) (D₁ : Seq Δ₁ A) (D₂ : Seq Δ₂ B) : Seq Δ (A.tensor B)
+  | tensorL (s : Split₁ Δ (A.tensor B) Δ') (D : Seq (Δ'.cons A |>.cons B) C) : Seq Δ C
+  | plusR₁ (D : Seq Δ A) : Seq Δ (A.plus B)
+  | plusR₂ (D : Seq Δ B) : Seq Δ (.plus A B)
+  | plusL (s : Split₁ Δ (A.plus B) Δ') (D₁ : Seq (Δ'.cons A) C) (D₂ : Seq (Δ'.cons B) C) : Seq Δ C
+  | withR (D₁ : Seq Δ A) (D₂ : Seq Δ B) : Seq Δ (A.with B)
+  | withL₁ (s : Split₁ Δ (A.with B) Δ') (D : Seq (Δ'.cons A) C) : Seq Δ C
+  | withL₂ (s : Split₁ Δ (.with A B) Δ') (D : Seq (Δ'.cons B) C) : Seq Δ C
+  | lolliR (D : Seq (Δ.cons A) B) : Seq Δ (A.lolli B)
+  | lolliL (s : Split₁ Δ (A.lolli B) Δ') (s' : Split Δ' Δ₁ Δ₂) (D₁ : Seq Δ₁ A) (D₂ : Seq (Δ₂.cons B) C) : Seq Δ C
 
-def Seq.rename (γ : Subst Hyp Γ Γ') {A} : (D : Seq Γ A) → Seq Γ' A
-  | id => let .cons s .mk .nil := γ; let .refl _ := s.eq_triv₁; id
-  | oneR => let .nil := γ; oneR
-  | oneL s D => let ⟨_, s, γ⟩ := γ.split₁ s; oneL s (D.rename γ)
-  | zeroL s => let ⟨_, s, _⟩ := γ.split₁ s; zeroL s
+class SCJudge (J) extends Judge J where
+  cut (s : Split Δ Δ₁ Δ₂) (D' : J Δ₁ A) (D : ∀ {Δ}, (s : Split₁ Δ A Δ₂) → SC.Seq Δ C) : SC.Seq Δ C
+
+instance Hyp.scJudge : SCJudge Hyp where
+  cut s D' D := D (let .mk := D'; .ofSplit s)
+
+namespace SC
+
+def Seq.subst [j : SCJudge J] {Δ Δ'} (δ : Subst J Δ Δ') {A} : (D : Seq Δ A) → Seq Δ' A
+  | id => let .cons s D' .nil := δ; j.cut s D' fun | .here => id
+  | oneR => let .nil := δ; oneR
+  | oneL s D => let ⟨_, _, s, D', δ⟩ := δ.split₁ s; j.cut s D' fun s => oneL s (D.subst δ)
+  | zeroL s => let ⟨_, _, s, D', _⟩ := δ.split₁ s; j.cut s D' zeroL
   | topR => topR
-  | tensorR s D₁ D₂ => let ⟨_, _, s, γ₁, γ₂⟩ := γ.split s; tensorR s (D₁.rename γ₁) (D₂.rename γ₂)
-  | tensorL s D => let ⟨_, s, γ⟩ := γ.split₁ s; tensorL s (D.rename γ.lift.lift)
-  | plusR₁ D => plusR₁ (D.rename γ)
-  | plusR₂ D => plusR₂ (D.rename γ)
-  | plusL s D₁ D₂ => let ⟨_, s, γ⟩ := γ.split₁ s; plusL s (D₁.rename γ.lift) (D₂.rename γ.lift)
-  | withR D₁ D₂ => withR (D₁.rename γ) (D₂.rename γ)
-  | withL₁ s D => let ⟨_, s, γ⟩ := γ.split₁ s; withL₁ s (D.rename γ.lift)
-  | withL₂ s D => let ⟨_, s, γ⟩ := γ.split₁ s; withL₂ s (D.rename γ.lift)
-  | lolliR D => lolliR (D.rename γ.lift)
-  | lolliL s s' D₁ D₂ => let ⟨_, s, γ⟩ := γ.split₁ s; let ⟨_, _, s', γ₁, γ₂⟩ := γ.split s'; lolliL s s' (D₁.rename γ₁) (D₂.rename γ₂.lift)
+  | tensorR s D₁ D₂ => let ⟨_, _, s, δ₁, δ₂⟩ := δ.split s; tensorR s (D₁.subst δ₁) (D₂.subst δ₂)
+  | tensorL s D => let ⟨_, _, s, D', δ⟩ := δ.split₁ s; j.cut s D' fun s => tensorL s (D.subst δ.lift.lift)
+  | plusR₁ D => plusR₁ (D.subst δ)
+  | plusR₂ D => plusR₂ (D.subst δ)
+  | plusL s D₁ D₂ => let ⟨_, _, s, D', δ⟩ := δ.split₁ s; j.cut s D' fun s => plusL s (D₁.subst δ.lift) (D₂.subst δ.lift)
+  | withR D₁ D₂ => withR (D₁.subst δ) (D₂.subst δ)
+  | withL₁ s D => let ⟨_, _, s, D', δ⟩ := δ.split₁ s; j.cut s D' fun s => withL₁ s (D.subst δ.lift)
+  | withL₂ s D => let ⟨_, _, s, D', δ⟩ := δ.split₁ s; j.cut s D' fun s => withL₂ s (D.subst δ.lift)
+  | lolliR D => lolliR (D.subst δ.lift)
+  | lolliL s s' D₁ D₂ => let ⟨_, _, s, D', δ⟩ := δ.split₁ s; let ⟨_, _, s', δ₁, δ₂⟩ := δ.split s'; j.cut s D' fun s => lolliL s s' (D₁.subst δ₁) (D₂.subst δ₂.lift)
 
 def Seq.id' : Seq (.cons .nil A) A :=
   match A with
@@ -326,18 +292,18 @@ def Seq.id' : Seq (.cons .nil A) A :=
   | .lolli .. => lolliR (lolliL (.there .here) (.cons₁ .nil) id' id')
 
 @[simp]
-def Seq.sizeOf : (D : Seq Γ A) → Nat
+def Seq.sizeOf : (D : Seq Δ A) → Nat
   | id | oneR | zeroL _ | topR => 0
   | oneL _ D | tensorL _ D | plusR₁ D | plusR₂ D | withL₁ _ D | withL₂ _ D | lolliR D => D.sizeOf + 1
   | tensorR _ D₁ D₂ | plusL _ D₁ D₂ | withR D₁ D₂ | lolliL _ _ D₁ D₂ => D₁.sizeOf + D₂.sizeOf + 1
 
 @[simp]
-theorem Seq.sizeOf_rename (γ : Subst Hyp Γ Γ') {A} (D : Seq Γ A) : (D.rename γ).sizeOf = D.sizeOf := by
-  induction D generalizing Γ' <;> simp! only [*]
-  case id => let .cons s .mk .nil := γ; let .refl _ := s.eq_triv₁; rfl
-  case oneR => let .nil := γ; rfl
+theorem Seq.sizeOf_subst (δ : Subst Hyp Δ Δ') {A} (D : Seq Δ A) : (D.subst δ).sizeOf = D.sizeOf := by
+  induction D generalizing Δ' <;> simp! only [*]
+  case id => let .cons s .mk .nil := δ; let .refl _ := s.eq_triv₁; rfl
+  case oneR => let .nil := δ; rfl
 
-def Seq.cut (s : Split Γ Γ₁ Γ₂) : (D : Seq Γ₁ A) → (E : Seq (Γ₂.cons A) C) → Seq Γ C
+def Seq.cut (s : Split Δ Δ₁ Δ₂) : (D : Seq Δ₁ A) → (E : Seq (Δ₂.cons A) C) → Seq Δ C
   | D, id => let .refl _ := s.eq_triv₁; D
   | oneR, oneL .here E => let .refl _ := s.eq_triv₂; E
   | tensorR s' D₁ D₂, tensorL .here E => let ⟨_, s, s'⟩ := s.shift₁ s'; cut s D₁ (cut s'.cons₂ D₂ E)
@@ -358,26 +324,23 @@ def Seq.cut (s : Split Γ Γ₁ Γ₂) : (D : Seq Γ₁ A) → (E : Seq (Γ₂.c
   | _, topR => topR
   | D, tensorR (.cons₁ s') E₁ E₂ => let ⟨_, s, s'⟩ := s.flip.shift₁ s'.flip; tensorR s.flip (cut s'.flip D E₁) E₂
   | D, tensorR (.cons₂ s') E₁ E₂ => let ⟨_, s, s'⟩ := s.flip.shift₁ s'; tensorR s E₁ (cut s'.flip D E₂)
-  | D, tensorL (.there s') E => let ⟨_, s, s'⟩ := s.flip.shift₁ s'.toSplit; tensorL (.ofSplit s) (cut s'.flip.cons₂.cons₂ D (E.rename .exchange₂))
+  | D, tensorL (.there s') E => let ⟨_, s, s'⟩ := s.flip.shift₁ s'.toSplit; tensorL (.ofSplit s) (cut s'.flip.cons₂.cons₂ D (E.subst .exchange₂))
   | D, plusR₁ E => plusR₁ (cut s D E)
   | D, plusR₂ E => plusR₂ (cut s D E)
-  | D, plusL (.there s') E₁ E₂ => let ⟨_, s, s'⟩ := s.flip.shift₁ s'.toSplit; plusL (.ofSplit s) (cut s'.flip.cons₂ D (E₁.rename .exchange)) (cut s'.flip.cons₂ D (E₂.rename .exchange))
+  | D, plusL (.there s') E₁ E₂ => let ⟨_, s, s'⟩ := s.flip.shift₁ s'.toSplit; plusL (.ofSplit s) (cut s'.flip.cons₂ D (E₁.subst .exchange)) (cut s'.flip.cons₂ D (E₂.subst .exchange))
   | D, withR E₁ E₂ => withR (cut s D E₁) (cut s D E₂)
-  | D, withL₁ (.there s') E => let ⟨_, s, s'⟩ := s.flip.shift₁ s'.toSplit; withL₁ (.ofSplit s) (cut s'.flip.cons₂ D (E.rename .exchange))
-  | D, withL₂ (.there s') E => let ⟨_, s, s'⟩ := s.flip.shift₁ s'.toSplit; withL₂ (.ofSplit s) (cut s'.flip.cons₂ D (E.rename .exchange))
-  | D, lolliR E => lolliR (cut s.cons₂ D (E.rename .exchange))
+  | D, withL₁ (.there s') E => let ⟨_, s, s'⟩ := s.flip.shift₁ s'.toSplit; withL₁ (.ofSplit s) (cut s'.flip.cons₂ D (E.subst .exchange))
+  | D, withL₂ (.there s') E => let ⟨_, s, s'⟩ := s.flip.shift₁ s'.toSplit; withL₂ (.ofSplit s) (cut s'.flip.cons₂ D (E.subst .exchange))
+  | D, lolliR E => lolliR (cut s.cons₂ D (E.subst .exchange))
   | D, lolliL (.there s') (.cons₁ s'') E₁ E₂ => let ⟨_, s, s'⟩ := s.flip.shift₁ s'.toSplit; let ⟨_, s', s''⟩ := s'.shift₁ s''.flip; lolliL (.ofSplit s) s'.flip (cut s''.flip D E₁) E₂
-  | D, lolliL (.there s') (.cons₂ s'') E₁ E₂ => let ⟨_, s, s'⟩ := s.flip.shift₁ s'.toSplit; let ⟨_, s', s''⟩ := s'.shift₁ s''; lolliL (.ofSplit s) s' E₁ (cut s''.flip.cons₂ D (E₂.rename .exchange))
+  | D, lolliL (.there s') (.cons₂ s'') E₁ E₂ => let ⟨_, s, s'⟩ := s.flip.shift₁ s'.toSplit; let ⟨_, s', s''⟩ := s'.shift₁ s''; lolliL (.ofSplit s) s' E₁ (cut s''.flip.cons₂ D (E₂.subst .exchange))
   termination_by D E => (A, D.sizeOf, E.sizeOf)
 
-def Seq.multicut : (γ : Subst Seq Γ₂ Γ₂') → ∀ {Γ₁ A}, (D : Seq (.append Γ₁ Γ₂) A) → Seq (Γ₁.append Γ₂') A
-  | .nil, _, _, D => D
-  | .cons s D' γ, _, _, D => (Ctx.append_append ▸ multicut γ (cut (.append₂ (.flip .mkAppend)) D' D)).rename (.append .id s.toSubst)
+instance Seq.scJudge : SCJudge Seq where
+  hyp := id'
+  cut s D' D := cut s D' (D .here)
 
-def Seq.subst (γ : Subst Seq Γ Γ') {A} (D : Seq Γ A) : Seq Γ' A :=
-  (Ctx.nil_append ▸ multicut γ (Γ₁ := .nil) (A := A) (Ctx.nil_append ▸ D) :)
-
-def Seq.toVerif : (D : Seq Γ A) → VU.Verif Γ A
+def Seq.toVerif : (D : Seq Δ A) → VU.Verif Δ A
   | id => .uv .hyp
   | oneR => .oneI
   | oneL s D => .oneE s.toSplit .hyp D.toVerif
@@ -396,7 +359,7 @@ def Seq.toVerif : (D : Seq Γ A) → VU.Verif Γ A
 
 end SC
 
-def ND.True.toSeq : (D : True Γ A) → SC.Seq Γ A
+def ND.True.toSeq : (D : True Δ A) → SC.Seq Δ A
   | hyp => .id'
   | oneI => .oneR
   | oneE s D D₁ => .cut s D.toSeq (.oneL .here D₁.toSeq)
@@ -413,5 +376,5 @@ def ND.True.toSeq : (D : True Γ A) → SC.Seq Γ A
   | lolliI D => .lolliR D.toSeq
   | lolliE s D D₁ => .cut s D.toSeq (.lolliL .here .triv₁ D₁.toSeq .id')
 
-def VU.Verif.subst' (γ : Subst Verif Γ Γ') {A} (D : Verif Γ A) : Verif Γ' A :=
-  (D.toTrue.toSeq.subst (γ.map ⟨fun D => D.toTrue.toSeq⟩)).toVerif
+def VU.Verif.subst' (δ : Subst Verif Δ Δ') {A} (D : Verif Δ A) : Verif Δ' A :=
+  (D.toTrue.toSeq.subst (δ.map fun D => D.toTrue.toSeq)).toVerif
