Logic/Propositional/Structural/Classical.lean
@@ -1,5 +1,3 @@
-namespace Logic.Propositional.Structural.Classical
-
 opaque BasePropn : Type
 
 inductive Propn
@@ -18,58 +16,55 @@ inductive Hyp (A : Propn) : (Γ : Ctx) → Type
   | here : Hyp A (.cons Γ A)
   | there (u : Hyp A Γ) : Hyp A (Γ.cons B)
 
-def Rename (Γ Γ' : Ctx) : Type :=
+def Renaming (Γ Γ' : Ctx) : Type :=
   ∀ ⦃A⦄, (u : Hyp A Γ) → Hyp A Γ'
 
-def Rename.id : Rename Γ Γ
+def Renaming.id : Renaming Γ Γ
   | _, u => u
 
-def Rename.weakening : Rename Γ (Γ.cons A)
+def Renaming.weakening : Renaming Γ (Γ.cons A)
   | _ => .there
 
-def Rename.contraction (u : Hyp A Γ) : Rename (Γ.cons A) Γ
-  | _, .here => u
-  | _, .there u => u
-
-def Rename.exchange : Rename (Ctx.cons Γ A |>.cons B) (Γ.cons B |>.cons A)
+def Renaming.exchange : Renaming (Ctx.cons Γ A |>.cons B) (Γ.cons B |>.cons A)
   | _, .here => .there .here
   | _, .there .here => .here
   | _, .there (.there u) => u.there.there
 
-def Rename.lift (γ : Rename Γ Γ') {A} : Rename (Γ.cons A) (Γ'.cons A)
+def Renaming.lift (γ : Renaming Γ Γ') {A} : Renaming (Γ.cons A) (Γ'.cons A)
   | _, .here => .here
   | _, .there u => (γ u).there
 
--- Sequent Calculus
+/-! Sequent Calculus -/
+
 namespace SC
 
-inductive Seq : (Γ : Ctx) → (Δ : Ctx) → Type
-  | id (u : Hyp (.base P) Γ) (v : Hyp (.base P) Δ) : Seq Γ Δ
-  | trueR (v : Hyp .true Δ) : Seq Γ Δ
-  | falseL (u : Hyp .false Γ) : Seq Γ Δ
-  | notR (v : Hyp A.not Δ) (D : Seq (Γ.cons A) Δ) : Seq Γ Δ
-  | notL (u : Hyp A.not Γ) (D : Seq Γ (Δ.cons A)) : Seq Γ Δ
-  | andR (v : Hyp (A.and B) Δ) (D₁ : Seq Γ (Δ.cons A)) (D₂ : Seq Γ (Δ.cons B)) : Seq Γ Δ
-  | andL₁ (u : Hyp (A.and B) Γ) (D : Seq (Γ.cons A) Δ) : Seq Γ Δ
-  | andL₂ (u : Hyp (.and A B) Γ) (D : Seq (Γ.cons B) Δ) : Seq Γ Δ
-  | orR₁ (v : Hyp (A.or B) Δ) (D : Seq Γ (Δ.cons A)) : Seq Γ Δ
-  | orR₂ (v : Hyp (.or A B) Δ) (D : Seq Γ (Δ.cons B)) : Seq Γ Δ
-  | orL (u : Hyp (A.or B) Γ) (D₁ : Seq (Γ.cons A) Δ) (D₂ : Seq (Γ.cons B) Δ) : Seq Γ Δ
+inductive Seq : (Γ₁ Γ₂ : Ctx) → Type
+  | id (u : Hyp (.base P) Γ₁) (v : Hyp (.base P) Γ₂) : Seq Γ₁ Γ₂
+  | trueR (v : Hyp .true Γ₂) : Seq Γ₁ Γ₂
+  | falseL (u : Hyp .false Γ₁) : Seq Γ₁ Γ₂
+  | notR (v : Hyp A.not Γ₂) (D : Seq (Γ₁.cons A) Γ₂) : Seq Γ₁ Γ₂
+  | notL (u : Hyp A.not Γ₁) (D : Seq Γ₁ (Γ₂.cons A)) : Seq Γ₁ Γ₂
+  | andR (v : Hyp (A.and B) Γ₂) (D₁ : Seq Γ₁ (Γ₂.cons A)) (D₂ : Seq Γ₁ (Γ₂.cons B)) : Seq Γ₁ Γ₂
+  | andL₁ (u : Hyp (A.and B) Γ₁) (D : Seq (Γ₁.cons A) Γ₂) : Seq Γ₁ Γ₂
+  | andL₂ (u : Hyp (.and A B) Γ₁) (D : Seq (Γ₁.cons B) Γ₂) : Seq Γ₁ Γ₂
+  | orR₁ (v : Hyp (A.or B) Γ₂) (D : Seq Γ₁ (Γ₂.cons A)) : Seq Γ₁ Γ₂
+  | orR₂ (v : Hyp (.or A B) Γ₂) (D : Seq Γ₁ (Γ₂.cons B)) : Seq Γ₁ Γ₂
+  | orL (u : Hyp (A.or B) Γ₁) (D₁ : Seq (Γ₁.cons A) Γ₂) (D₂ : Seq (Γ₁.cons B) Γ₂) : Seq Γ₁ Γ₂
 
-def Seq.rename (γ : Rename Γ Γ') (δ : Rename Δ Δ') : (D : Seq Γ Δ) → Seq Γ' Δ'
-  | id u v => id (γ u) (δ v)
-  | trueR v => trueR (δ v)
-  | falseL u => falseL (γ u)
-  | notR v D => notR (δ v) (D.rename γ.lift δ)
-  | notL u D => notL (γ u) (D.rename γ δ.lift)
-  | andR v D₁ D₂ => andR (δ v) (D₁.rename γ δ.lift) (D₂.rename γ δ.lift)
-  | andL₁ u D => andL₁ (γ u) (D.rename γ.lift δ)
-  | andL₂ u D => andL₂ (γ u) (D.rename γ.lift δ)
-  | orR₁ v D => orR₁ (δ v) (D.rename γ δ.lift)
-  | orR₂ v D => orR₂ (δ v) (D.rename γ δ.lift)
-  | orL u D₁ D₂ => orL (γ u) (D₁.rename γ.lift δ) (D₂.rename γ.lift δ)
+def Seq.rename (γ₁ : Renaming Γ₁ Γ₁') (γ₂ : Renaming Γ₂ Γ₂') : (D : Seq Γ₁ Γ₂) → Seq Γ₁' Γ₂'
+  | id u v => id (γ₁ u) (γ₂ v)
+  | trueR v => trueR (γ₂ v)
+  | falseL u => falseL (γ₁ u)
+  | notR v D => notR (γ₂ v) (D.rename γ₁.lift γ₂)
+  | notL u D => notL (γ₁ u) (D.rename γ₁ γ₂.lift)
+  | andR v D₁ D₂ => andR (γ₂ v) (D₁.rename γ₁ γ₂.lift) (D₂.rename γ₁ γ₂.lift)
+  | andL₁ u D => andL₁ (γ₁ u) (D.rename γ₁.lift γ₂)
+  | andL₂ u D => andL₂ (γ₁ u) (D.rename γ₁.lift γ₂)
+  | orR₁ v D => orR₁ (γ₂ v) (D.rename γ₁ γ₂.lift)
+  | orR₂ v D => orR₂ (γ₂ v) (D.rename γ₁ γ₂.lift)
+  | orL u D₁ D₂ => orL (γ₁ u) (D₁.rename γ₁.lift γ₂) (D₂.rename γ₁.lift γ₂)
 
-def Seq.id' (u : Hyp A Γ) (v : Hyp A Δ) : Seq Γ Δ :=
+def Seq.id' (u : Hyp A Γ₁) (v : Hyp A Γ₂) : Seq Γ₁ Γ₂ :=
   match A with
   | .base _ => id u v
   | .true => trueR v
@@ -79,19 +74,18 @@ def Seq.id' (u : Hyp A Γ) (v : Hyp A Δ) : Seq Γ Δ :=
   | .or .. => orL u (orR₁ v (id' .here .here)) (orR₂ v (id' .here .here))
 
 @[simp]
-def Seq.sizeOf : (D : Seq Γ A) → Nat
+def Seq.sizeOf : (D : Seq Γ₁ Γ₂) → Nat
   | id .. | trueR _ | falseL _ => 0
   | notR _ D | notL _ D | andL₁ _ D | andL₂ _ D | orR₁ _ D | orR₂ _ D => D.sizeOf + 1
   | andR _ D₁ D₂ | orL _ D₁ D₂ => D₁.sizeOf + D₂.sizeOf + 1
 
 @[simp]
-theorem Seq.sizeOf_rename (γ : Rename Γ Γ') (δ : Rename Δ Δ') (D : Seq Γ Δ) : (D.rename γ δ).sizeOf = D.sizeOf :=
-  by induction D generalizing Γ' Δ' <;> simp! only [*]
+theorem Seq.sizeOf_rename (γ₁ : Renaming Γ₁ Γ₁') (γ₂ : Renaming Γ₂ Γ₂') (D : Seq Γ₁ Γ₂) : (D.rename γ₁ γ₂).sizeOf = D.sizeOf :=
+  by induction D generalizing Γ₁' Γ₂' <;> simp! only [*]
 
-def Seq.cut : (D : Seq Γ (Δ.cons A)) → (E : Seq (Γ.cons A) Δ) → Seq Γ Δ
-  | .id u .here, E => E.rename (.contraction u) .id
+def Seq.cut : (D : Seq Γ₁ (Γ₂.cons A)) → (E : Seq (Γ₁.cons A) Γ₂) → Seq Γ₁ Γ₂
+  | .id u .here, .id .here v => .id u v
   | .id u (.there v), _ => .id u v
-  | D, .id .here v => D.rename .id (.contraction v)
   | _, .id (.there u) v => .id u v
   | D@(notR .here D₁), E@(notL .here E₁) => cut (cut (D.rename .id (.lift .weakening)) E₁) (cut D₁ (E.rename (.lift .weakening) .id))
   | D@(andR .here D₁ _), E@(andL₁ .here E₁) => cut (cut (D₁.rename .id .exchange) (E.rename .id .weakening)) (cut (D.rename .weakening .id) (E₁.rename .exchange .id))
